case-studies/kathrin/coq-ext/Chapter9/preservation.v
@@ -1,8 +1,9 @@
 (** ** Typing, Context Morphism Lemmas, and Preservation *)
 
 Require Import core core_axioms fintype fintype_axioms.
-Import ScopedNotations.
 From Chapter9 Require Export reduction.
+Import ScopedNotations.
+
 
 (** A context *)
 Definition ctx n := fin n -> ty.
@@ -18,6 +19,11 @@ Inductive has_type {n} (Gamma : ctx n) : tm n -> ty -> Prop :=
     has_type Gamma M (Fun T S) ->
     has_type Gamma N T ->
     has_type Gamma (app M N) S.
+
+Create HintDb has_type_db.
+
+#[ export ]
+ Hint Constructors has_type : has_type_db.
 Notation "Gamma |- M : T" := (has_type Gamma M T) (at level 20, M at level 99).
 
 
@@ -28,21 +34,20 @@ Definition ltc {k k'} (Gamma: ctx k) (Delta: ctx k') rho := forall x, Delta (rho
 Lemma typing_ren n k (Gamma: ctx n) (Delta: ctx k) (rho: fin n -> fin k) (M: tm n) T :
   ltc Gamma Delta rho  -> Gamma |- M : T ->  Delta |- (M⟨rho⟩) : T.
 Proof.
-  intros C H. revert k Delta rho C. induction H; intros; cbn; eauto using has_type.
+  intros C H. revert k Delta rho C. induction H; intros; cbn; eauto with has_type_db.
   - unfold ltc in C. rewrite <- C. constructor.
   - constructor. apply IHhas_type. asimpl. unfold ltc. auto_case.
-  - econstructor; eauto.
 Qed.
 
 Lemma typing_inst n k (Gamma: ctx n) (Delta: ctx k) (sigma: fin n -> tm k) (M: tm n) T :
   (forall x, Delta |- sigma x : Gamma x) -> Gamma |- M : T ->  Delta |- (M[sigma]) : T.
 Proof.
-  intros C H. revert k Delta sigma C. induction H; intros; asimpl; eauto using has_type.
-  - apply C.
+  intros C H. revert k Delta sigma C. induction H; intros; asimpl; eauto with has_type_db.
+  (* - apply C. *)
   - constructor. apply IHhas_type. auto_case.
     + eapply typing_ren; eauto. intros. unfold ltc. now asimpl.
     + constructor.
-  - econstructor; eauto.
+  (* - econstructor; eauto. *)
 Qed.
 
 Lemma preservation k (Gamma: ctx k) M T :
