case-studies/kathrin/coq-ext/unscoped.v
@@ -51,19 +51,19 @@ Class Ren5 (X1 X2 X3 X4 X5 : Type) (Y Z : Type) :=
   ren5 : X1 -> X2 -> X3 -> X4 -> X5 -> Y -> Z.
 
 Module RenNotations.
-  Notation "s ⟨ xi1 ⟩" := (ren1 xi1 s) (at level 7, left associativity, format "s  ⟨ xi1 ⟩") : subst_scope.
+  Notation "s ⟨ xi1 ⟩" := (ren1 xi1 s) (at level 7, left associativity, format "s  ⟨ xi1 ⟩") : subst_scope'.
 
-  Notation "s ⟨ xi1 ; xi2 ⟩" := (ren2 xi1 xi2 s) (at level 7, left associativity, format "s  ⟨ xi1 ; xi2 ⟩") : subst_scope.
+  Notation "s ⟨ xi1 ; xi2 ⟩" := (ren2 xi1 xi2 s) (at level 7, left associativity, format "s  ⟨ xi1 ; xi2 ⟩") : subst_scope'.
 
-  Notation "s ⟨ xi1 ; xi2 ; xi3 ⟩" := (ren3 xi1 xi2 xi3 s) (at level 7, left associativity, format "s  ⟨ xi1 ; xi2 ; xi3 ⟩") : subst_scope.
+  Notation "s ⟨ xi1 ; xi2 ; xi3 ⟩" := (ren3 xi1 xi2 xi3 s) (at level 7, left associativity, format "s  ⟨ xi1 ; xi2 ; xi3 ⟩") : subst_scope'.
 
-  Notation "s ⟨ xi1 ; xi2 ; xi3 ; xi4 ⟩" := (ren4  xi1 xi2 xi3 xi4 s) (at level 7, left associativity, format "s  ⟨ xi1 ; xi2 ; xi3 ; xi4 ⟩") : subst_scope.
+  Notation "s ⟨ xi1 ; xi2 ; xi3 ; xi4 ⟩" := (ren4  xi1 xi2 xi3 xi4 s) (at level 7, left associativity, format "s  ⟨ xi1 ; xi2 ; xi3 ; xi4 ⟩") : subst_scope'.
 
-  Notation "s ⟨ xi1 ; xi2 ; xi3 ; xi4 ; xi5 ⟩" := (ren5  xi1 xi2 xi3 xi4 xi5 s) (at level 7, left associativity, format "s  ⟨ xi1 ; xi2 ; xi3 ; xi4 ; xi5 ⟩") : subst_scope.
+  Notation "s ⟨ xi1 ; xi2 ; xi3 ; xi4 ; xi5 ⟩" := (ren5  xi1 xi2 xi3 xi4 xi5 s) (at level 7, left associativity, format "s  ⟨ xi1 ; xi2 ; xi3 ; xi4 ; xi5 ⟩") : subst_scope'.
 
-  Notation "⟨ xi ⟩" := (ren1 xi) (at level 1, left associativity, format "⟨ xi ⟩") : fscope.
+  Notation "⟨ xi ⟩" := (ren1 xi) (at level 1, left associativity, format "⟨ xi ⟩") : fscope'.
 
-  Notation "⟨ xi1 ; xi2 ⟩" := (ren2 xi1 xi2) (at level 1, left associativity, format "⟨ xi1 ; xi2 ⟩") : fscope.
+  Notation "⟨ xi1 ; xi2 ⟩" := (ren2 xi1 xi2) (at level 1, left associativity, format "⟨ xi1 ; xi2 ⟩") : fscope'.
 End RenNotations.
 
 (** *** Type Classes for Substiution *)
@@ -84,9 +84,9 @@ Class Subst5 (X1 X2 X3 X4 X5 : Type) (Y Z: Type) :=
   subst5 : X1 -> X2 -> X3 -> X4 -> X5  -> Y  -> Z.
 
 Module SubstNotations.
-  Notation "s [ sigma ]" := (subst1 sigma s) (at level 7, left associativity, format "s '/' [ sigma ]") : subst_scope.
+  Notation "s [ sigma ]" := (subst1 sigma s) (at level 7, left associativity, format "s '/' [ sigma ]") : subst_scope'.
 
-  Notation "s [ sigma ; tau ]" := (subst2 sigma tau s) (at level 7, left associativity, format "s '/' [ sigma ; '/'  tau ]") : subst_scope.
+  Notation "s [ sigma ; tau ]" := (subst2 sigma tau s) (at level 7, left associativity, format "s '/' [ sigma ; '/'  tau ]") : subst_scope'.
 End SubstNotations.
 
 (** *** Type Class for Variables *)
@@ -98,15 +98,17 @@ Instance idsRen : Var nat nat := id.
 
 (** ** Proofs for the substitution primitives. *)
 
-Arguments funcomp {X Y Z} (g)%fscope (f)%fscope.
+Arguments funcomp {X Y Z} (g)%fscope' (f)%fscope'.
 
 Module CombineNotations.
-  Notation "f >> g" := (funcomp g f) (at level 50) : fscope.
+  Notation "f >> g" := (funcomp g f) (at level 50) : fscope'.
 
-  Notation "s .: sigma" := (scons s sigma) (at level 55, sigma at next level, right associativity) : subst_scope.
+  Notation "s .: sigma" := (scons s sigma) (at level 55, sigma at next level, right associativity) : subst_scope'.
 
-  Open Scope fscope.
-  Open Scope subst_scope.
+  (* Open Scope fscope. *)
+  Open Scope fscope'.
+  (* Open Scope subst_scope. *)
+  Open Scope subst_scope'.
 End CombineNotations.
 
 Import CombineNotations.
@@ -133,14 +135,14 @@ Module UnscopedNotations.
   
   (* Notation "s , sigma" := (scons s sigma) (at level 60, format "s ,  sigma", right associativity) : subst_scope. *)
 
-  Notation "s '..'" := (scons s ids) (at level 1, format "s ..") : subst_scope.
+  Notation "s '..'" := (scons s ids) (at level 1, format "s ..") : subst_scope'.
 
-  Notation "↑" := (shift) : subst_scope.
+  Notation "↑" := (shift) : subst_scope'.
 
   #[ global ]
-  Open Scope fscope.
+  Open Scope fscope'.
   #[ global ]
-  Open Scope subst_scope.
+  Open Scope subst_scope'.
 End UnscopedNotations.
 
 (** ** Tactics for unscoped syntax *)
